new/proof/go_etcd_io/etcd/api/v3/etcdserverpb.v
@@ -1,0 +1,36 @@
+Require Export New.code.go_etcd_io.etcd.api.v3.etcdserverpb.
+Require Export New.generatedproof.go_etcd_io.etcd.api.v3.etcdserverpb.
+Require Export New.proof.proof_prelude.
+
+Section wps.
+Context `{hG: heapGS Σ, !ffi_semantics _ _}.
+Context `{!globalsGS Σ} {go_ctx : GoContext}.
+#[global] Instance : IsPkgInit etcdserverpb := define_is_pkg_init True%I.
+
+(* FIXME: annoying to even state axioms about marshalling this stuff.
+   Want to turn the protobuf data into Gallina.
+ *)
+Axiom InternalRaftRequestC : Type.
+Axiom own_InternalRaftRequest :
+  ∀ (req : etcdserverpb.InternalRaftRequest.t) (req_abs : InternalRaftRequestC), iProp Σ.
+Axiom is_RaftRequest_marshalled : ∀ (req_abs : InternalRaftRequestC) (data : list w8), Prop.
+
+Axiom own_InternalRaftRequest_new_header :
+  ∀ req hdr_ptr (hdr : etcdserverpb.RequestHeader.t) req_abs,
+  own_InternalRaftRequest req req_abs -∗
+  hdr_ptr ↦ hdr -∗
+  ∃ req_abs',
+    own_InternalRaftRequest (req <| etcdserverpb.InternalRaftRequest.Header' := hdr_ptr |>) req_abs'.
+
+Axiom wp_InternalRaftRequest__Marshal : ∀ m_ptr m msg,
+  {{{ is_pkg_init etcdserverpb ∗ m_ptr ↦ m ∗ own_InternalRaftRequest m msg }}}
+    m_ptr @ (ptrT.id etcdserverpb.InternalRaftRequest.id) @ "Marshal" #()
+  {{{ dAtA_sl (err : error.t), RET (#dAtA_sl, #err);
+      m_ptr ↦ m ∗
+      if decide (err = interface.nil) then
+        ∃ dAtA, dAtA_sl ↦*□ dAtA ∧ ⌜ is_RaftRequest_marshalled msg dAtA ⌝
+      else
+        ⌜ dAtA_sl = slice.nil ⌝
+  }}}.
+
+End wps.
